\section {Rytter Algorithm for Graph Input} 

Main idea is to adopt algorithm from~\cite{Rytter} for CFPQ.
It should be possible to perform adoptation for arbitrary CFPQ, but we are interested in case of Dyck queryes.

We introduce an example and try to explain key steps.
As far as example for graph and query introduced in the previous section is too big, we use another input data.

Let the input grammar is 
\begin{align*}
S & \rightarrow a \ S \ b \ 
\\
S & \rightarrow a \ b
\end{align*}

The input grammar in CNF is 
\begin{align*}
S   & \rightarrow A \ S_1
\\
S_1 & \rightarrow S \ B
\\
S   & \rightarrow A \ B
\\
A   & \rightarrow a
\\
B   & \rightarrow b
\end{align*}


Let the input graph is
\\
\begin{tikzpicture}[shorten >=1pt,node distance=2cm,on grid,auto] 
   \node[state] (q_1)   {$1$}; 
   \node[state] (q_2) [above right=of q_1] {$2$}; 
   \node[state] (q_3) [right=of q_2] {$3$}; 
   \node[state] (q_4) [right=of q_3] {$4$};
    \path[->] 
    (q_1) edge  node {a} (q_2)          
    (q_2) edge  node {a} (q_3)
    (q_3) edge  node {a} (q_1)
    (q_3) edge[bend left, above]  node {b} (q_4)
    (q_4) edge[bend left, below]  node {b} (q_3);
\end{tikzpicture}

  

The \emph{IMPLIED} relation:
\begin{figure*}
\begin{align*} % S -> A B
(B,2,3)  & \Rightarrow (S,1,3)  & (B,2,4)  & \Rightarrow (S,1,4)  & (B,2,2)  & \Rightarrow (S,1,2) & (B,2,1)  & \Rightarrow (S,1,1)
\\
(B,3,4)  & \Rightarrow (S,2,4)  & (B,3,3)  & \Rightarrow (S,2,3)  & (B,3,2)  & \Rightarrow (S,2,2) & (B,3,1)  & \Rightarrow (S,2,1)
\\
(B,1,2)  & \Rightarrow (S,3,2)  & (B,1,3)  & \Rightarrow (S,3,3)  & (B,1,4)  & \Rightarrow (S,3,4) & (B,1,1)  & \Rightarrow (S,3,1)
\\ %S -> A S1
(S_1,2,3)  & \Rightarrow (S,1,3) & (S_1,2,4)  & \Rightarrow (S,1,4) & (S_1,2,2)  & \Rightarrow (S,1,2) & (S_1,2,1)  & \Rightarrow (S,1,1)
\\
(S_1,3,4)  & \Rightarrow (S,2,4)  & (S_1,3,3)  & \Rightarrow (S,2,3)  & (S_1,3,2)  & \Rightarrow (S,2,2) & (S_1,3,1)  & \Rightarrow (S,2,1)
\\
(S_1,1,2)  & \Rightarrow (S,3,2)  &  (S_1,1,3) & \Rightarrow (S,3,3)  & (S_1,1,4)  & \Rightarrow (S,3,4)  & (S_1,1,1)  & \Rightarrow (S,3,1)
\\ % S -> A B
(A,2,3)  & \Rightarrow (S,2,4)    &  (A,1,3) & \Rightarrow (S,1,4)    & (A,3,3)  & \Rightarrow (S,3,4)    & (A,4,3)  & \Rightarrow (S,4,4)
\\
(A,3,4)  & \Rightarrow (S,3,3)    &  (A,4,4) & \Rightarrow (S,4,3)    & (A,2,4)  & \Rightarrow (S,2,3)    & (A,1,4)  & \Rightarrow (S,1,3)
\\ % S1 -> S B
(S,2,3)  & \Rightarrow (S_1,2,4)  &  (S,1,3) & \Rightarrow (S_1,1,4)  & (S,3,3)  & \Rightarrow (S_1,3,4)  & (S,4,3)  & \Rightarrow (S_1,4,4)
\\
(S,3,4)  & \Rightarrow (S_1,3,3)  &  (S,4,4) & \Rightarrow (S_1,4,3)  & (S,2,4)  & \Rightarrow (S_1,2,3)  & (S,1,4)  & \Rightarrow (S_1,1,3)
\end{align*}
\end{figure*}


Grid:
\begin{figure*}  

\begin{tikzpicture}[shorten >=1pt,node distance=4.5cm,on grid,auto] 
   \node[state] (q_1)   {$1$}; 
   \node[state] (q_2) [right=of q_1] {\tiny{$2$}}; 
   \node[state] (q_3) [right=of q_2] {\tiny{$3$ (B)}}; 
   \node[state] (q_4) [right=of q_3] {\tiny{$4$}};

   \node[state] (q_5) [below=of q_1] {\tiny{$5$ (A)}};
   \node[state] (q_6) [right=of q_5] {\tiny{$6$}};
   \node[state] (q_7) [right=of q_6] {\tiny{$7$}};
   \node[state] (q_8) [right=of q_7] {\tiny{$8$ (B)}};
  
   \node[state] (q_9) [below=of q_5] {\tiny{$9$}};
   \node[state] (q_10) [right=of q_9] {\tiny{$10$}};
   \node[state] (q_11) [right=of q_10] {\tiny{$11$ (A)}};
   \node[state] (q_12) [right=of q_11] {\tiny{$12$}};
   
   \node[state] (q_13) [below=of q_9] {\tiny{$13$}};
   \node[state] (q_14) [right=of q_13] {\tiny{$14$ (A)}};
   \node[state] (q_15) [right=of q_14] {\tiny{$15$}};
   \node[state] (q_16) [right=of q_15] {\tiny{$16$}};

    \path[->] 
     
     (q_11) edge  node {\tiny{$\{(B,S);(S_1,S)\}$}} (q_15)
     (q_12) edge  node {\tiny{$\{(B,S);(S_1,S)\}$}} (q_16)
     (q_10) edge  node {\tiny{$\{(B,S);(S_1,S)\}$}} (q_14)
     (q_9) edge  node {\tiny{$\{(B,S);(S_1,S)\}$}} (q_13)

     (q_8) edge  node {\tiny{$\{(B,S);(S_1,S)\}$}} (q_12)
     (q_7) edge  node {\tiny{$\{(B,S);(S_1,S)\}$}} (q_11)
     (q_6) edge  node {\tiny{$\{(B,S);(S_1,S)\}$}} (q_10)
     (q_5) edge  node {\tiny{$\{(B,S);(S_1,S)\}$}} (q_9)

     (q_14) edge[bend left]  node {\tiny{$\{(B,S);(S_1,S)\}$}} (q_6)
     (q_13) edge[bend left]  node {\tiny{$\{(B,S);(S_1,S)\}$}} (q_5)
     (q_15) edge[bend left]  node {\tiny{$\{(B,S);(S_1,S)\}$}} (q_7)
     (q_16) edge[bend left]  node {\tiny{$\{(B,S);(S_1,S)\}$}} (q_8)

     (q_11) edge[bend left]  node {\tiny{$\{(A,S);(S,S_1)\}$}} (q_12)
     (q_15) edge[bend left]  node {\tiny{$\{(A,S);(S,S_1)\}$}} (q_16)
     (q_7) edge[bend left]  node {\tiny{$\{(A,S);(S,S_1)\}$}} (q_8)
     (q_3) edge[bend left]  node {\tiny{$\{(A,S);(S,S_1)\}$}} (q_4)

     (q_8) edge[bend left]  node {\tiny{$\{(A,S);(S,S_1)\}$}} (q_7)
     (q_4) edge[bend left]  node {\tiny{$\{(A,S);(S,S_1)\}$}} (q_3)
     (q_12) edge[bend left]  node {\tiny{$\{(A,S);(S,S_1)\}$}} (q_11)
     (q_16) edge[bend left]  node {\tiny{$\{(A,S);(S,S_1)\}$}} (q_15)

     
     ;
\end{tikzpicture}
\end{figure*}  

We should introduce the \emph{id} implication such that for every $A \in \text{IMPLIED}$
\begin{itemize}
\item $\text{\emph{id}} \times A = A \times \text{\emph{id}}$
\end{itemize}

In order to compute transitive closure in logarithmic time we add self-loop with weight $\{\text{\emph{id}}\}$ to each vertex.

\begin{figure*}  
\begin{tikzpicture}[shorten >=1pt,node distance=4.5cm,on grid,auto] 
   \node[state] (q_1)   {$1$}; 
   \node[state] (q_2) [right=of q_1] {\tiny{$2$}}; 
   \node[state] (q_3) [right=of q_2] {\tiny{$3$ (B)}}; 
   \node[state] (q_4) [right=of q_3] {\tiny{$4$}};

   \node[state] (q_5) [below=of q_1] {\tiny{$5$ (A)}};
   \node[state] (q_6) [right=of q_5] {\tiny{$6$}};
   \node[state] (q_7) [right=of q_6] {\tiny{$7$}};
   \node[state] (q_8) [right=of q_7] {\tiny{$8$ (B)}};
  
   \node[state] (q_9) [below=of q_5] {\tiny{$9$}};
   \node[state] (q_10) [right=of q_9] {\tiny{$10$}};
   \node[state] (q_11) [right=of q_10] {\tiny{$11$ (A)}};
   \node[state] (q_12) [right=of q_11] {\tiny{$12$}};
   
   \node[state] (q_13) [below=of q_9] {\tiny{$13$}};
   \node[state] (q_14) [right=of q_13] {\tiny{$14$ (A)}};
   \node[state] (q_15) [right=of q_14] {\tiny{$15$}};
   \node[state] (q_16) [right=of q_15] {\tiny{$16$}};

    \path[->] 
     
     (q_11) edge  node {\tiny{$\{(B,S);(S_1,S)\}$}} (q_15)
     (q_12) edge  node {\tiny{$\{(B,S);(S_1,S)\}$}} (q_16)
     (q_10) edge  node {\tiny{$\{(B,S);(S_1,S)\}$}} (q_14)
     (q_9) edge  node {\tiny{$\{(B,S);(S_1,S)\}$}} (q_13)

     (q_8) edge  node {\tiny{$\{(B,S);(S_1,S)\}$}} (q_12)
     (q_7) edge  node {\tiny{$\{(B,S);(S_1,S)\}$}} (q_11)
     (q_6) edge  node {\tiny{$\{(B,S);(S_1,S)\}$}} (q_10)
     (q_5) edge  node {\tiny{$\{(B,S);(S_1,S)\}$}} (q_9)

     (q_14) edge[bend left]  node {\tiny{$\{(B,S);(S_1,S)\}$}} (q_6)
     (q_13) edge[bend left]  node {\tiny{$\{(B,S);(S_1,S)\}$}} (q_5)
     (q_15) edge[bend left]  node {\tiny{$\{(B,S);(S_1,S)\}$}} (q_7)
     (q_16) edge[bend left]  node {\tiny{$\{(B,S);(S_1,S)\}$}} (q_8)

     (q_11) edge[bend left]  node {\tiny{$\{(A,S);(S,S_1)\}$}} (q_12)
     (q_15) edge[bend left]  node {\tiny{$\{(A,S);(S,S_1)\}$}} (q_16)
     (q_7) edge[bend left]  node {\tiny{$\{(A,S);(S,S_1)\}$}} (q_8)
     (q_3) edge[bend left]  node {\tiny{$\{(A,S);(S,S_1)\}$}} (q_4)

     (q_8) edge[bend left]  node {\tiny{$\{(A,S);(S,S_1)\}$}} (q_7)
     (q_4) edge[bend left]  node {\tiny{$\{(A,S);(S,S_1)\}$}} (q_3)
     (q_12) edge[bend left]  node {\tiny{$\{(A,S);(S,S_1)\}$}} (q_11)
     (q_16) edge[bend left]  node {\tiny{$\{(A,S);(S,S_1)\}$}} (q_15)

     (q_1) edge[loop] node {\tiny{$\{\text{\emph{id}}\}$}} (q_1)
     (q_2) edge[loop] node {\tiny{$\{\text{\emph{id}}\}$}} (q_2)
     (q_3) edge[loop] node {\tiny{$\{\text{\emph{id}}\}$}} (q_3)
     (q_4) edge[loop] node {\tiny{$\{\text{\emph{id}}\}$}} (q_4)
     (q_5) edge[loop] node {\tiny{$\{\text{\emph{id}}\}$}} (q_5)
     (q_6) edge[loop] node {\tiny{$\{\text{\emph{id}}\}$}} (q_6)
     (q_7) edge[loop] node {\tiny{$\{\text{\emph{id}}\}$}} (q_7)
     (q_8) edge[loop] node {\tiny{$\{\text{\emph{id}}\}$}} (q_8)
     (q_9) edge[loop] node {\tiny{$\{\text{\emph{id}}\}$}} (q_9)
     (q_10) edge[loop] node {\tiny{$\{\text{\emph{id}}\}$}} (q_10)
     (q_11) edge[loop] node {\tiny{$\{\text{\emph{id}}\}$}} (q_11)
     (q_12) edge[loop] node {\tiny{$\{\text{\emph{id}}\}$}} (q_12)
     (q_13) edge[loop] node {\tiny{$\{\text{\emph{id}}\}$}} (q_13)
     (q_14) edge[loop] node {\tiny{$\{\text{\emph{id}}\}$}} (q_14)
     (q_15) edge[loop] node {\tiny{$\{\text{\emph{id}}\}$}} (q_15)
     (q_16) edge[loop] node {\tiny{$\{\text{\emph{id}}\}$}} (q_16)
     

     
     ;
\end{tikzpicture}

\end{figure*}  

Note that our graph is a Cartezian product of tho graph $H$ and $V$ with respective matrices.

$H=$
\begin{align*}
\begin{pmatrix}
      \{ \text{\emph{id}} \} & \varnothing            & \varnothing            & \varnothing            \\
      \varnothing            & \{ \text{\emph{id}} \} & \varnothing            & \varnothing            \\
      \varnothing            & \varnothing            & \{ \text{\emph{id}} \} & \{(A,S);(S,S_1)\}      \\
      \varnothing            & \varnothing            & \{(A,S);(S,S_1)\}      & \{ \text{\emph{id}} \}  \\
\end{pmatrix}
\end{align*}



$V=$
\begin{align*}
\begin{pmatrix}
      \{ \text{\emph{id}} \}       & \varnothing       & \varnothing       & \varnothing  \\ 
      \varnothing       & \{ \text{\emph{id}} \}       & \{(B,S);(S_1,S)\} & \varnothing  \\
      \varnothing       & \varnothing       & \{ \text{\emph{id}} \}       & \{(B,S);(S_1,S)\}  \\
      \varnothing       & \{(B,S);(S_1,S)\} & \varnothing       & \{ \text{\emph{id}} \}  \\
\end{pmatrix}
\end{align*}


Matrix of $G = V \otimes I + I \otimes H$ where $I$ is identity matrix of size $n \times n$ and $\otimes$ is a Kronecker product.


One step is APSP (or transitive closure) of $G$.
It can be computed as $(V \otimes I + I \otimes H)^{(n^2)}$.
Now we should check validity of nonterminals.
It can be don by multiplication of vector $x$ and $M$.
$x*(V^{(n^2)} \otimes I + V^{(n^2)} \otimes H^{(n^2)} + I \otimes H^{(n^2)}) = $
$x*V^{(n^2)} \otimes I + x*V^{(n^2)} \otimes H^{(n^2)} + x * I \otimes H^{(n^2)} $.




$X=$
\begin{align*}
\begin{pmatrix}
      \varnothing            & \varnothing            & \{ (\perp,B) \}            & \varnothing            \\
      \{ (\perp,A) \}        & \varnothing            & \varnothing                & \{ (\perp,B) \}            \\
      \varnothing            & \varnothing            & \{ (\perp,A) \}            & \varnothing      \\
      \varnothing            & \{ (\perp,A) \}            & \varnothing      & \varnothing  \\
\end{pmatrix}
\end{align*}

$X^T=$
\begin{align*}
\begin{pmatrix}
      \varnothing            & \{ (\perp,A) \}        & \varnothing            & \varnothing            \\
      \varnothing            & \varnothing            & \varnothing                & \{ (\perp,A) \}            \\
      \{ (\perp,B) \}        & \varnothing            & \{ (\perp,A) \}            & \varnothing      \\
      \varnothing            & \{ (\perp,B) \}            & \varnothing      & \varnothing  \\
\end{pmatrix}
\end{align*}